src/cbor/pulse/raw/everparse/CBOR.Pulse.Raw.EverParse.Det.Compare.fsti
@@ -1,0 +1,30 @@
+module CBOR.Pulse.Raw.EverParse.Det.Compare
+#lang-pulse
+include CBOR.Spec.Raw.Format
+open CBOR.Spec.Raw.EverParse
+include CBOR.Pulse.Raw.EverParse.Validate
+open CBOR.Pulse.Raw.EverParse.Type
+open CBOR.Pulse.Raw.EverParse.Match
+open CBOR.Pulse.Raw.Compare.Base
+open Pulse.Lib.Pervasives
+
+module SZ = FStar.SizeT
+module I16 = FStar.Int16
+
+inline_for_extraction
+val impl_cbor_compare
+  (f64: squash SZ.fits_u64)
+  (x1: cbor_raw)
+  (x2: cbor_raw)
+  (#pm1: perm)
+  (#v1: Ghost.erased raw_data_item)
+  (#pm2: perm)
+  (#v2: Ghost.erased raw_data_item)
+: stt I16.t
+    (cbor_raw_match pm1 x1 v1 **
+     cbor_raw_match pm2 x2 v2)
+    (fun res ->
+      cbor_raw_match pm1 x1 v1 **
+      cbor_raw_match pm2 x2 v2 **
+      pure (same_sign (I16.v res) (cbor_compare v1 v2)))
+
